Field as inductive selector

LeanCourse/Memory.lean
@@ -1,41 +1,44 @@
 import Aesop
 
 set_option autoImplicit true
+variable {IdType : Type}
 
-structure IdT (β γ δ : Type) where
-  pId  : δ
-  flds : List (β ⊕ γ)
+@[aesop safe [constructors, cases]]
+inductive FieldSelector (β γ : Type) where
+  | valS  (valS : β)
+  | idS (idS : γ)
+  deriving DecidableEq
 
-inductive ValT (α β γ δ : Type) where
+structure IdT (β γ IdType : Type) where
+  pId  : IdType
+  flds : List (FieldSelector β γ)
+
+inductive ValT (α β γ IdType : Type) where
   | val (val : α)
-  | id  (id : IdT β γ δ)
+  | id  (id : IdT β γ IdType)
 
--- def ValT α β γ δ := α ⊕ IdT β γ δ
-
-open Sum
-
-instance [DecidableEq β] [DecidableEq γ] [DecidableEq δ] : DecidableEq (IdT β γ δ) := by
+instance [DecidableEq β] [DecidableEq γ] [DecidableEq IdType] : DecidableEq (IdT β γ IdType) := by
   rintro ⟨a1, b1⟩ ⟨a2, b2⟩
   simp
-  have h : Decidable ((⟨a1, b1⟩ : δ × List (β ⊕ γ)) = ⟨a2, b2⟩)  := by exact (inferInstanceAs _)
+  have h : Decidable ((⟨a1, b1⟩ : IdType × List (FieldSelector β γ)) = ⟨a2, b2⟩)  := by exact (inferInstanceAs _)
   cases h
   . apply isFalse; aesop
   . apply isTrue; aesop
 
-inductive Memory (α β γ δ : Type) where
+inductive Memory (α β γ IdType : Type) where
   | mtm
-  | write (mem : Memory α β γ δ) (id : IdT β γ δ) (fld : β ⊕ γ) (val : ValT α β γ δ)
-  | add   (mem : Memory α β γ δ) (id : δ)
+  | write (mem : Memory α β γ IdType) (id : IdT β γ IdType) (fld : FieldSelector β γ) (val : ValT α β γ IdType)
+  | add   (mem : Memory α β γ IdType) (id : IdType)
 
 namespace Memory
 
-@[simp] def read [DecidableEq β] [DecidableEq γ] [DecidableEq δ] [Inhabited α] (mem : Memory α β γ δ) (id : IdT β γ δ) (fld : β ⊕ γ) : ValT α β γ δ :=
+@[simp] def read [DecidableEq β] [DecidableEq γ] [DecidableEq IdType] [Inhabited α] (mem : Memory α β γ IdType) (id : IdT β γ IdType) (fld : FieldSelector β γ) : ValT α β γ IdType :=
   match mem, id with
   | .mtm, _ => .val default
   | .write mem idM fldM val, _ => if idM = id && fldM = fld then val else read mem id fld
-  | .add mem pId, ⟨idd, ids⟩ => if pId = idd
+  | .add mem pId, ⟨idd, valS⟩ => if pId = idd
     then (match fld with
-      | inl _ => .val default
-      | inr _ => .id ⟨idd, fld :: ids⟩
+      | .valS  _ => .val default
+      | .idS _ => .id ⟨idd, fld :: valS⟩
       )
     else read mem id fld
