LeanCourse/Storage.lean
@@ -1,5 +1,7 @@
 import Aesop
 
+import LeanCourse.Memory
+
 set_option autoImplicit true
 
 open Sum
@@ -7,12 +9,12 @@ open Sum
 inductive Value (α β γ : Type) where
   | mtst
   | var   (val : α)
-  | store (st : Value α β γ) (k : β ⊕ γ) (v : Value α β γ)
+  | store (st : Value α β γ) (k : FieldSelector β γ) (v : Value α β γ)
 
 open Value
 
 @[simp] def save [DecidableEq β] [DecidableEq γ]
-  (st : Value α β γ) (fields : List (β ⊕ γ)) (v : Value α β γ) : Value α β γ :=
+  (st : Value α β γ) (fields : List (FieldSelector β γ)) (v : Value α β γ) : Value α β γ :=
   match st, fields with
   | mtst, [] => v
   | mtst, k :: rest => store mtst k $ save mtst rest v
@@ -21,7 +23,7 @@ open Value
   | store st k v', xs@(k' :: ys) =>
     if k = k' then store st k (save v' ys v) else store (save st xs v) k v'
 
-@[simp] def select [DecidableEq β] [DecidableEq γ] (st : Value α β γ) (k : β ⊕ γ) : Value α β γ :=
+@[simp] def select [DecidableEq β] [DecidableEq γ] (st : Value α β γ) (k : FieldSelector β γ) : Value α β γ :=
   match st with
   | mtst => mtst
   | var _ => mtst
@@ -31,19 +33,19 @@ open Value
   match st with
   | mtst => true
   | var _ => false
-  | store st (inl _) (var _) => isStruct st
-  | store _  (inr _) (var _) => false
-  | store st (inr _) st2 => And (isStruct st) (isStruct st2)
+  | store st (.valS _) (var _) => isStruct st
+  | store _  (.idS _) (var _) => false
+  | store st (.idS _) st2 => And (isStruct st) (isStruct st2)
   | _ => false
 
 theorem structInside {st : Value α β γ} {k} {v} (wf : isStruct (store st k v)) : isStruct st := by
   cases v <;> aesop
 
-theorem structInsideR {st : Value α β γ} {k} {v} (wf : isStruct (store st (inr k) v)) : isStruct v := by
+theorem structInsideR {st : Value α β γ} {k} {v} (wf : isStruct (store st (.idS k) v)) : isStruct v := by
   cases v <;> aesop
 
 theorem selectSave [DecidableEq β] [DecidableEq γ]
-  (st : Value α β γ) (k : β ⊕ γ) (path : List (β ⊕ γ)) (v : Value α β γ) (k' : β ⊕ γ) (wf : isStruct st := by simp) :
+  (st : Value α β γ) (k : FieldSelector β γ) (path : List (FieldSelector β γ)) (v : Value α β γ) (k' : FieldSelector β γ) (wf : isStruct st := by simp) :
   select (save st (k :: path) v) k' =
   (if k = k' then save (select st k') path v else select st k') := by
   induction st with
