LeanCourse/StorageToMemory.lean
@@ -15,10 +15,10 @@ structure State (α β γ δ : Type) where
   match st with
   | mtst => mem
   | var _ => by aesop
-  | store st (inl k) .mtst => by aesop
-  | store st (inl k) (var x) => write (copyStAux mem id st (by aesop)) id (inl k) (.val x)
-  | store st (inl k) (store a b c) => by aesop
-  | store st x@(inr _) v =>
+  | store st (.valS k) .mtst => by aesop
+  | store st (.valS k) (var x) => write (copyStAux mem id st (by aesop)) id (.valS k) (.val x)
+  | store st (.valS k) (store a b c) => by aesop
+  | store st x@(.idS _) v =>
       let copyInt := copyStAux mem id st (by induction v <;> aesop)
       copyStAux copyInt ⟨id.1, x :: id.2⟩ v $ by
         induction v
@@ -39,14 +39,14 @@ theorem not_suff_imp_not_cons_suff (l1 l2 : List α) (x : α) :
 
 
 @[simp] theorem readSkip [DecidableEq β] [DecidableEq γ] [DecidableEq δ] [Inhabited α]
-  (mem : Memory α β γ δ) (pId pIdR : δ) (st : Value α β γ) (fxsL fxsR : List (β ⊕ γ)) (fld : β ⊕ γ)
+  (mem : Memory α β γ δ) (pId pIdR : δ) (st : Value α β γ) (fxsL fxsR : List (FieldSelector β γ)) (fld : FieldSelector β γ)
   (wf : isStruct st := by simp) (pIdDiff : ¬pId = pIdR ⊕' pId = pIdR ×' ¬ fxsL <:+ (fld :: fxsR))
   : read (copyStAux mem ⟨pId, fxsL⟩ st wf) ⟨ pIdR , fxsR ⟩ fld = read mem ⟨ pIdR, fxsR⟩ fld :=
 
   match st with
   | mtst => by aesop
   | var _ => by simp at wf
-  | store st (inl f) (var x) => by
+  | store st (.valS f) (var x) => by
     have h := readSkip mem pId pIdR st fxsL fxsR fld (by aesop) (by aesop)
     induction pIdDiff
     . unfold copyStAux
@@ -68,13 +68,13 @@ theorem not_suff_imp_not_cons_suff (l1 l2 : List α) (x : α) :
       have h3 := List.suffix_cons fld fxsL
       have _ := notSuff.2 h3
       contradiction
-  | store st (inr f) v => by
+  | store st (.idS f) v => by
     have _ := structInside wf
     have stInR := structInsideR wf
     have _ := readSkip mem pId pIdR st fxsL fxsR fld (by aesop) (by aesop)
-    have _ := not_suff_imp_not_cons_suff fxsL (fld :: fxsR) (inr f)
+    have _ := not_suff_imp_not_cons_suff fxsL (fld :: fxsR) (.idS f)
     let copyAuxVal := copyStAux mem ⟨pId, fxsL⟩ st (by aesop)
-    have _ := readSkip copyAuxVal pId pIdR v (inr f :: fxsL) fxsR fld stInR
+    have _ := readSkip copyAuxVal pId pIdR v (.idS f :: fxsL) fxsR fld stInR
     aesop
 
 inductive SameVal {α β γ δ : Type} : ValT α β γ δ → Value α β γ → Prop where
@@ -84,8 +84,8 @@ inductive SameVal {α β γ δ : Type} : ValT α β γ δ → Value α β γ →
 open SameVal
 
 theorem readFind [DecidableEq β] [DecidableEq γ] [DecidableEq δ] [Inhabited α]
-  (mem : Memory α β γ δ) (id : δ) (st : Value α β γ) (fxs : List (β ⊕ γ)) (f : β) (wf : isStruct st := by simp)
-  : SameVal (read (copySt mem id st wf) ⟨id, []⟩ (inl f)) (select st (inl f)) :=
+  (mem : Memory α β γ δ) (id : δ) (st : Value α β γ) (fxs : List (FieldSelector β γ)) (f : β) (wf : isStruct st := by simp)
+  : SameVal (read (copySt mem id st wf) ⟨id, []⟩ (.valS f)) (select st (.valS f)) :=
   match st with
   | mtst => by
     simp
@@ -93,8 +93,8 @@ theorem readFind [DecidableEq β] [DecidableEq γ] [DecidableEq δ] [Inhabited �
   | var _ => by
     unfold isStruct at wf
     aesop
-  | store st idS@(inr idSS) sv => by
-    have copy := readSkip (copyStAux (add mem id) ⟨id, []⟩ st (structInside wf)) id id sv [.inr idSS] [] (inl f) (structInsideR wf)
+  | store st valS@(.idS valSS) sv => by
+    have copy := readSkip (copyStAux (add mem id) ⟨id, []⟩ st (structInside wf)) id id sv [.idS valSS] [] (.valS f) (structInsideR wf)
       (.inr ⟨rfl, fun x => by
         have sub := List.IsSuffix.sublist x
         cases sub
@@ -105,7 +105,7 @@ theorem readFind [DecidableEq β] [DecidableEq γ] [DecidableEq δ] [Inhabited �
     rw [copy]
     have readFindd := readFind mem id st [] f (structInside wf)
     apply readFindd
-  | store st (inl idS) sv@(var _) => by
+  | store st (.valS valS) sv@(var _) => by
     have readFindd := readFind mem id st fxs f (structInside wf)
     simp
     split
@@ -114,24 +114,24 @@ theorem readFind [DecidableEq β] [DecidableEq γ] [DecidableEq δ] [Inhabited �
 
 @[simp] theorem skipIdRead [DecidableEq β] [DecidableEq γ] [DecidableEq δ] [Inhabited α]
   (mem : Memory α β γ δ) (idC idR : IdT β γ δ) (st : Value α β γ) (fld : γ) (wf : isStruct st := by simp)
-  : read (copyStAux mem idC st wf) idR (inr fld) = read mem idR (inr fld) :=
+  : read (copyStAux mem idC st wf) idR (.idS fld) = read mem idR (.idS fld) :=
   match st with
   | mtst => by aesop
   | var _ => by
     unfold isStruct at wf
     aesop
-  | store st (inl f) (var _) => by
+  | store st (.valS f) (var _) => by
     have _ := skipIdRead mem idC idR st fld (structInside wf)
     aesop
-  | store st (inr id) v => by
+  | store st (.idS id) v => by
     have wfIn := structInside wf
     have _ := skipIdRead mem idC idR st fld wfIn
-    have _ := skipIdRead (copyStAux mem idC st wfIn) ⟨idC.1, inr id :: idC.2⟩ idR v fld (structInsideR wf)
+    have _ := skipIdRead (copyStAux mem idC st wfIn) ⟨idC.1, .idS id :: idC.2⟩ idR v fld (structInsideR wf)
     aesop
 
 @[simp] theorem readGetId [DecidableEq β] [DecidableEq γ] [DecidableEq δ] [Inhabited α]
-  (mem : Memory α β γ δ) (pId : δ) (st : Value α β γ) (fxs : List (β ⊕ γ)) (fld : γ) (wf : isStruct st := by simp)
-  : read (copySt mem pId st wf) ⟨pId, fxs⟩ (inr fld) = .id ⟨pId, inr fld :: fxs⟩ := by
+  (mem : Memory α β γ δ) (pId : δ) (st : Value α β γ) (fxs : List (FieldSelector β γ)) (fld : γ) (wf : isStruct st := by simp)
+  : read (copySt mem pId st wf) ⟨pId, fxs⟩ (.idS fld) = .id ⟨pId, .idS fld :: fxs⟩ := by
   have h := skipIdRead (add mem pId) ⟨pId, []⟩ ⟨pId, fxs⟩ st fld wf
   unfold copySt
   rw [h]
